# The Sequence s_n = (2^(2n+1) + 1)/3: A Complete Mathematical Analysis

**Abstract:** We provide a rigorous mathematical analysis of the integer sequence defined by s_n = (2^(2n+1) + 1)/3 for n ≥ 0. We prove that this formula is well-defined, establish a linear recurrence relation, and analyze divisibility properties. All results are presented with complete proofs.

## 1. Introduction and Preliminaries

### Definition 1.1 (2-adic valuation)
For a nonzero integer m, the 2-adic valuation ν_2(m) is the largest integer k such that 2^k divides m. We define ν_2(0) = ∞.

### Definition 1.2 (2-adic absolute value)
For a nonzero integer m, the 2-adic absolute value is |m|_2 = 2^(-ν_2(m)). We define |0|_2 = 0.

### Lemma 1.3
For all integers n ≥ 0, we have 2^(2n+1) ≡ 2 (mod 3).

**Proof:** We have 2 ≡ -1 (mod 3), so 2^(2n+1) = 2·(2^2)^n = 2·4^n. Since 4 ≡ 1 (mod 3), we get 2^(2n+1) ≡ 2·1^n = 2 ≡ -1 (mod 3). Therefore 2^(2n+1) + 1 ≡ 0 (mod 3). □

## 2. Main Results

### Theorem 2.1 (Well-defined sequence)
The sequence s_n = (2^(2n+1) + 1)/3 consists of positive integers for all n ≥ 0.

**Proof:** By Lemma 1.3, 3 divides 2^(2n+1) + 1, so s_n is an integer. Since 2^(2n+1) > 0, we have s_n > 0. □

### Theorem 2.2 (Explicit values)
The first terms of the sequence are:
- s_0 = 1
- s_1 = 3  
- s_2 = 11
- s_3 = 43
- s_4 = 171

**Proof:** Direct computation:
- s_0 = (2^1 + 1)/3 = 3/3 = 1
- s_1 = (2^3 + 1)/3 = 9/3 = 3
- s_2 = (2^5 + 1)/3 = 33/3 = 11
- s_3 = (2^7 + 1)/3 = 129/3 = 43
- s_4 = (2^9 + 1)/3 = 513/3 = 171 □

### Theorem 2.3 (Recurrence relation)
For all n ≥ 0, we have s_{n+1} = 4s_n - 1.

**Proof:**
Starting from the definition:
s_{n+1} = (2^(2(n+1)+1) + 1)/3 = (2^(2n+3) + 1)/3

We can rewrite 2^(2n+3) = 4·2^(2n+1). Therefore:
s_{n+1} = (4·2^(2n+1) + 1)/3

From the definition of s_n, we have 3s_n = 2^(2n+1) + 1, which gives 2^(2n+1) = 3s_n - 1.

Substituting:
s_{n+1} = (4(3s_n - 1) + 1)/3 = (12s_n - 4 + 1)/3 = (12s_n - 3)/3 = 4s_n - 1 □

### Theorem 2.4 (Modular inverse property)
For all n ≥ 0, s_n is the unique integer with 0 < s_n < 2^(2n+1) satisfying 3s_n ≡ 1 (mod 2^(2n+1)).

**Proof:**
From the definition, 3s_n = 2^(2n+1) + 1, so 3s_n - 1 = 2^(2n+1).
This means 3s_n ≡ 1 (mod 2^(2n+1)).

Since s_n = (2^(2n+1) + 1)/3 < (2^(2n+1) + 2^(2n+1))/3 = (2·2^(2n+1))/3 < 2^(2n+1), we have 0 < s_n < 2^(2n+1).

For uniqueness: Suppose 3t ≡ 1 (mod 2^(2n+1)) with 0 < t < 2^(2n+1).
Then 3(s_n - t) ≡ 0 (mod 2^(2n+1)).
Since gcd(3, 2^(2n+1)) = 1 (as 3 is odd and 2^(2n+1) is a power of 2), we have s_n ≡ t (mod 2^(2n+1)).
Since both s_n and t lie in the interval (0, 2^(2n+1)), we must have s_n = t. □

### Theorem 2.5 (Divisibility by powers of 2)
For all n ≥ 0, s_n divides 2^(4n+2) - 1.

**Proof:**
We have 3s_n = 2^(2n+1) + 1, so 2^(2n+1) ≡ -1 (mod s_n).
Squaring both sides: (2^(2n+1))^2 ≡ 1 (mod s_n).
Therefore 2^(4n+2) ≡ 1 (mod s_n), which means s_n | (2^(4n+2) - 1). □

### Theorem 2.6 (Congruence modulo 8)
For n = 0: s_0 = 1 ≡ 1 (mod 8)
For n = 1: s_1 = 3 ≡ 3 (mod 8)  
For n ≥ 2: s_n ≡ 3 (mod 8)

**Proof:**
For n ≥ 2, we have 2n + 1 ≥ 5, so 2^(2n+1) ≡ 0 (mod 32).
Therefore 2^(2n+1) + 1 ≡ 1 (mod 32).

We need to find s_n = (2^(2n+1) + 1)/3 modulo 8.
Since 2^(2n+1) + 1 ≡ 1 (mod 32), we can write 2^(2n+1) + 1 = 32k + 1 for some integer k.

We need 32k + 1 ≡ 0 (mod 3), which gives k ≡ 1 (mod 3).
So k = 3m + 1 for some integer m, and 2^(2n+1) + 1 = 32(3m + 1) + 1 = 96m + 33.

Therefore s_n = (96m + 33)/3 = 32m + 11 ≡ 11 ≡ 3 (mod 8). □

## 3. Convergence in the 2-adic Integers

### Theorem 3.1 (Cauchy sequence)
The sequence {s_n} is Cauchy with respect to the 2-adic metric.

**Proof:**
For m > n ≥ 0:
s_m - s_n = (2^(2m+1) + 1)/3 - (2^(2n+1) + 1)/3 = (2^(2m+1) - 2^(2n+1))/3 = 2^(2n+1)(2^(2(m-n)) - 1)/3

Since 2^(2(m-n)) - 1 is odd for m > n (as 2^k - 1 is odd for all k ≥ 1), and 3 is odd, the denominator contributes no factors of 2.
Therefore ν_2(s_m - s_n) = 2n + 1.

This gives |s_m - s_n|_2 = 2^(-(2n+1)) → 0 as n → ∞. □

## 4. Base-4 Representation

### Theorem 4.1
For n ≥ 1, in base-4 notation: s_n consists of (n-1) digits of 2 followed by a single digit 3.

**Proof by induction:**

Base case (n=1): s_1 = 3 = 3₄ ✓

Inductive step: Assume s_n has (n-1) twos followed by a three in base 4.
This means s_n = 2(4^(n-1) + 4^(n-2) + ... + 4 + 1) + 1 = 2·(4^n - 1)/(4 - 1) + 1 = (2·4^n - 2 + 3)/3 = (2·4^n + 1)/3.

Now s_{n+1} = 4s_n - 1 = 4·(2·4^n + 1)/3 - 1 = (8·4^n + 4 - 3)/3 = (8·4^n + 1)/3 = (2·4^(n+1) + 1)/3.

This has the form required for n+1, completing the induction. □

## 5. Open Questions

1. How many terms s_n are prime numbers?
2. Can we characterize all prime divisors of s_n for given n?
3. What is the growth rate of the largest prime factor of s_n?

## 6. Conclusion

We have provided a complete mathematical characterization of the sequence s_n = (2^(2n+1) + 1)/3 with rigorous proofs of all stated properties. The sequence has interesting connections to modular arithmetic and the 2-adic integers.

## References

[1] Hardy, G.H. and Wright, E.M. (2008). An Introduction to the Theory of Numbers. Oxford University Press.

[2] Koblitz, N. (1984). p-adic Numbers, p-adic Analysis, and Zeta-Functions. Springer-Verlag.